@prefix : <https://w3id.org/stav#> .
@prefix dct: <http://purl.org/dc/terms/> .
@prefix owl: <http://www.w3.org/2002/07/owl#> .
@prefix rdf: <http://www.w3.org/1999/02/22-rdf-syntax-ns#> .
@prefix xml: <http://www.w3.org/XML/1998/namespace> .
@prefix xsd: <http://www.w3.org/2001/XMLSchema#> .
@prefix odrl: <http://www.w3.org/ns/odrl/2/> .
@prefix rdfs: <http://www.w3.org/2000/01/rdf-schema#> .
@prefix skos: <http://www.w3.org/2004/02/skos/core#> .
@prefix spdx: <https://spdx.org/rdf/terms#> .
@prefix stap: <https://w3id.org/stap#> .
@base <https://w3id.org/stav#> .

<https://w3id.org/stav> rdf:type owl:Ontology ;
                         owl:versionIRI <https://w3id.org/stav/0.5> ;
                         owl:imports <http://spdx.org/rdf/terms/2.3> ,
                                     <https://w3id.org/stap/0.1> ;
                         dct:creator "Arthit Suriyawongkul" ;
                         dct:description "STAV represents AI system accountability concepts and relations."@en ;
                         dct:issued "2024-01-14T18:30:00" ;
                         dct:license "https://creativecommons.org/licenses/by/4.0/" ;
                         dct:modified "2024-04-16T14:30:00" ;
                         dct:publisher "ADAPT Centre, Trinity College Dublin" ;
                         dct:title "STAV" ;
                         rdfs:label "System Trustworthiness and Accountability Vocabulary"@en ;
                         owl:versionInfo 0.5 .

#################################################################
#    Annotation properties
#################################################################

###  http://purl.org/dc/terms/creator
dct:creator rdf:type owl:AnnotationProperty .


###  http://purl.org/dc/terms/description
dct:description rdf:type owl:AnnotationProperty .


###  http://purl.org/dc/terms/issued
dct:issued rdf:type owl:AnnotationProperty .


###  http://purl.org/dc/terms/license
dct:license rdf:type owl:AnnotationProperty .


###  http://purl.org/dc/terms/modified
dct:modified rdf:type owl:AnnotationProperty .


###  http://purl.org/dc/terms/publisher
dct:publisher rdf:type owl:AnnotationProperty .


###  http://purl.org/dc/terms/title
dct:title rdf:type owl:AnnotationProperty .


###  http://www.w3.org/2004/02/skos/core#definition
skos:definition rdf:type owl:AnnotationProperty .


###  http://www.w3.org/2004/02/skos/core#note
skos:note rdf:type owl:AnnotationProperty .


###  http://www.w3.org/ns/odrl/2/source
odrl:source rdf:type owl:AnnotationProperty .


#################################################################
#    Datatypes
#################################################################

###  https://w3id.org/stav#AISystemStatusType
:AISystemStatusType rdf:type rdfs:Datatype ;
                    owl:equivalentClass [ rdf:type rdfs:Datatype ;
                                          owl:oneOf [ rdf:type rdf:List ;
                                                      rdf:first "In service" ;
                                                      rdf:rest [ rdf:type rdf:List ;
                                                                 rdf:first "No longer placed on the market/in service" ;
                                                                 rdf:rest [ rdf:type rdf:List ;
                                                                            rdf:first "On the market" ;
                                                                            rdf:rest [ rdf:type rdf:List ;
                                                                                       rdf:first "Recalled" ;
                                                                                       rdf:rest rdf:nil
                                                                                     ]
                                                                          ]
                                                               ]
                                                    ]
                                        ] .


#################################################################
#    Object Properties
#################################################################

###  http://www.w3.org/ns/odrl/2/duty
odrl:duty rdf:type owl:ObjectProperty .


###  http://www.w3.org/ns/odrl/2/partOf
odrl:partOf rdf:type owl:ObjectProperty .


###  https://w3id.org/stav#hasAddress
:hasAddress rdf:type owl:ObjectProperty ;
            rdfs:subPropertyOf owl:topObjectProperty ;
            rdfs:domain :AIDeployer ,
                        :AIProvider .


###  https://w3id.org/stav#hasContactDetails
:hasContactDetails rdf:type owl:ObjectProperty ;
                   rdfs:subPropertyOf owl:topObjectProperty ;
                   rdfs:domain :AIDeployer ,
                               :AIProvider .


###  https://w3id.org/stav#hasName
:hasName rdf:type owl:ObjectProperty ;
         rdfs:domain :AIDeployer ,
                     :AIProvider ,
                     :AISystem ,
                     :AuthorisedRepresentative ,
                     :InformationSubmissionRepresentative ,
                     :MarketSurveillenceAuthority .


###  https://w3id.org/stav#onBehalfOf
:onBehalfOf rdf:type owl:ObjectProperty ;
            rdfs:subPropertyOf owl:topObjectProperty .


#################################################################
#    Classes
#################################################################

###  http://www.w3.org/ns/odrl/2/Action
odrl:Action rdf:type owl:Class .


###  http://www.w3.org/ns/odrl/2/Asset
odrl:Asset rdf:type owl:Class .


###  http://www.w3.org/ns/odrl/2/AssetCollection
odrl:AssetCollection rdf:type owl:Class .


###  http://www.w3.org/ns/odrl/2/Party
odrl:Party rdf:type owl:Class .


###  https://w3id.org/stap#InformationCreationObligation
stap:InformationCreationObligation rdf:type owl:Class .


###  https://w3id.org/stap#InformationSubmissionObligation
stap:InformationSubmissionObligation rdf:type owl:Class .


###  https://w3id.org/stav#AIDeployer
:AIDeployer rdf:type owl:Class ;
            rdfs:subClassOf odrl:Party ;
            rdfs:label "AI Deployer"@en ;
            skos:note "Article 3 (4)" ;
            odrl:source "https://eur-lex.europa.eu/legal-content/EN/TXT/HTML/?uri=CELEX:52021PC0206&from=EN" .


###  https://w3id.org/stav#AIProvider
:AIProvider rdf:type owl:Class ;
            rdfs:subClassOf odrl:Party ;
            rdfs:label "AI Provider"@en ;
            skos:note "Article 3 (2)" ;
            odrl:source "https://eur-lex.europa.eu/legal-content/EN/TXT/HTML/?uri=CELEX:52021PC0206&from=EN" .


###  https://w3id.org/stav#AISystem
:AISystem rdf:type owl:Class ;
          rdfs:subClassOf odrl:Asset ;
          rdfs:label "AI System"@en .


###  https://w3id.org/stav#AISystemStatus
:AISystemStatus rdf:type owl:Class ;
                rdfs:subClassOf odrl:Asset .


###  https://w3id.org/stav#AppliedStandards
:AppliedStandards rdf:type owl:Class ;
                  rdfs:subClassOf odrl:Asset ;
                  rdfs:comment "Annex IV (6)"@en ;
                  rdfs:label "Applied Standards"@en .


###  https://w3id.org/stav#AuthorisedRepresentative
:AuthorisedRepresentative rdf:type owl:Class ;
                          rdfs:subClassOf odrl:Party ;
                          rdfs:label "Authorised Representative"@en ;
                          skos:note "EU AI Act Annex VIII Section C (2)"@en .


###  https://w3id.org/stav#BaselineProcessDescription
:BaselineProcessDescription rdf:type owl:Class ;
                            rdfs:subClassOf odrl:Asset ;
                            rdfs:comment """Sec. 4. (a) (1) (A)
S. 2892: Algorithmic Accountability Act of 2023
https://www.govtrack.us/congress/bills/118/s2892/text/is#link=4_a_1_A"""@en ;
                            rdfs:label "Baseline Process Description"@en ;
                            skos:definition "Desciption of a previously existing decision-making process prior to the deployment of an AI/augmented decision process."@en .


###  https://w3id.org/stav#BeingNotHighRiskCriteria
:BeingNotHighRiskCriteria rdf:type owl:Class ;
                          rdfs:subClassOf odrl:Asset ;
                          rdfs:comment "Based on which criterion or criteria provided in Article 6(2a) the AI system is considered as not high-risk"@en ;
                          rdfs:label "Being Not High-Risk Criteria"@en ;
                          skos:note "EU AI Act Annex VIII Section C (5)"@en .


###  https://w3id.org/stav#BeingNotHighRiskGrounds
:BeingNotHighRiskGrounds rdf:type owl:Class ;
                         rdfs:subClassOf odrl:Asset ;
                         rdfs:comment "Short summary of the grounds for considering the AI system as not high-risk in application of the procedure under Article 6(2a)"@en ;
                         rdfs:label "Being Not High-Risk Grounds"@en ;
                         skos:note "EU AI Act Annex VIII Section C (6)"@en .


###  https://w3id.org/stav#ComponentsAndFunctionsSupportedDescription
:ComponentsAndFunctionsSupportedDescription rdf:type owl:Class ;
                                            rdfs:subClassOf odrl:Asset ;
                                            rdfs:comment "Description of the components and functions supported through this AI system"@en ;
                                            rdfs:label "Components And Functions Supported Description"@en ;
                                            skos:note "EU AI Act Annex VIII Section A (5)"@en .


###  https://w3id.org/stav#ConformityDeclaration
:ConformityDeclaration rdf:type owl:Class ;
                       rdfs:subClassOf odrl:Asset ;
                       rdfs:comment """Annex IV (7) EU AI Act

Can a text or an URL"""@en ;
                       rdfs:label "Conformity Declaration"@en .


###  https://w3id.org/stav#CurrentAndPotentialFutureImpacts
:CurrentAndPotentialFutureImpacts rdf:type owl:Class ;
                                  rdfs:subClassOf odrl:Asset ;
                                  rdfs:label "Current and Potential Future Impacts"@en ;
                                  skos:definition "Assessment and documentation of the current and potential future or downstream positive and negative impacts of a system or process."@en .


###  https://w3id.org/stav#DataMinimizationPractices
:DataMinimizationPractices rdf:type owl:Class ;
                           rdfs:subClassOf odrl:Asset ;
                           rdfs:label "Data Minimization Practices"@en ;
                           skos:definition "Assessment and documentation of the data minimization practices of a system or process and the duration for which the relevant identifying information and any resulting critical decision is stored."@en .


###  https://w3id.org/stav#DataProtectionImpactAssessmentDocumentation
:DataProtectionImpactAssessmentDocumentation rdf:type owl:Class ;
                                             rdfs:subClassOf :ImpactAssessmentDocumentation ;
                                             rdfs:comment "A summary of the data protection impact assessment carried out in accordance with Article 35 of Regulation (EU) 2016/679 or Article 27 of Directive (EU) 2016/680 as specified in paragraph 6 of Article 29 of this Regulation, where applicable."@en ;
                                             rdfs:label "Data Protection Impact Assessment Documentation"@en ;
                                             skos:note "EU AI Act Annex VIII Section B (7)"@en .


###  https://w3id.org/stav#DeploymentContext
:DeploymentContext rdf:type owl:Class ;
                   rdfs:subClassOf odrl:Asset ;
                   rdfs:comment """Sec. 203. (a) (2) (C)
S. 3312: Artificial Intelligence Research, Innovation, and Accountability Act of 2023
https://www.govtrack.us/congress/bills/118/s3312/text/is#link=II_203_a_2_C&nearest=id07706866948d4dc59792b34859a3afdf"""@en ;
                   rdfs:label "Deployment Context"@en .


###  https://w3id.org/stav#ExternalInteractionDescription
:ExternalInteractionDescription rdf:type owl:Class ;
                                rdfs:subClassOf odrl:Asset ;
                                rdfs:comment "EU AI Act Annex IV (1) (b)" ;
                                rdfs:label "External Interaction Description"@en ;
                                skos:definition "How the AI system interacts or can be used to interact with hardware or software that is not part of the AI system itself, where applicable."@en .


###  https://w3id.org/stav#FundamentalRightsImpactAssessmentDocumentation
:FundamentalRightsImpactAssessmentDocumentation rdf:type owl:Class ;
                                                rdfs:subClassOf :ImpactAssessmentDocumentation ;
                                                rdfs:comment "A summary of the findings of the fundamental rights impact assessment conducted in accordance with Article 29a."@en ;
                                                rdfs:label "Fundamental Rights Impact Assessment Documentation"@en ;
                                                skos:note "EU AI Act Annex VIII Section B (5)"@en .


###  https://w3id.org/stav#ImpactAssessmentDocumentation
:ImpactAssessmentDocumentation rdf:type owl:Class ;
                               rdfs:subClassOf odrl:AssetCollection ;
                               rdfs:comment """S. 2892: Algorithmic Accountability Act of 2023
Defined in Sec. 2. (12)
https://www.govtrack.us/congress/bills/118/s2892/text/is#link=2_12
and detailed in Sec. 4. (a)
https://www.govtrack.us/congress/bills/118/s2892/text/is#link=4_a

S. 3312: Artificial Intelligence Research, Innovation, and Accountability Act of 2023
Title II Sec. 206. (b)
https://www.govtrack.us/congress/bills/118/s3312/text/is#link=II_206_b"""@en ;
                               rdfs:label "Impact Assessment Documentation" .


###  https://w3id.org/stav#InformationSecurityMeasures
:InformationSecurityMeasures rdf:type owl:Class ;
                             rdfs:subClassOf odrl:Asset ;
                             rdfs:label "Information Security Measures"@en ;
                             skos:definition "Assessment of information security measures with respect to a system or process."@en .


###  https://w3id.org/stav#InformationSubmissionRepresentative
:InformationSubmissionRepresentative rdf:type owl:Class ;
                                     rdfs:subClassOf odrl:Party ;
                                     rdfs:label "Information Submission Representative"@en ;
                                     skos:note "EU AI Act Annex VIII Section C (1)"@en .


###  https://w3id.org/stav#InformationUsedBySystemDescription
:InformationUsedBySystemDescription rdf:type owl:Class ;
                                    rdfs:subClassOf odrl:Asset ;
                                    rdfs:comment "A basic and concise description of the information used by the system (data, inputs) and its operating logic"@en ;
                                    rdfs:label "Information Used By the System Description"@en ;
                                    skos:note "EU AI Act Annex VIII Section A (5a)"@en .


###  https://w3id.org/stav#InstallationInstructions
:InstallationInstructions rdf:type owl:Class ;
                          rdfs:subClassOf odrl:Asset ,
                                          [ rdf:type owl:Restriction ;
                                            owl:onProperty odrl:partOf ;
                                            owl:someValuesFrom :SystemGeneralDescription
                                          ] ;
                          rdfs:label "Installation Instructions"@en .


###  https://w3id.org/stav#InstructionsForUse
:InstructionsForUse rdf:type owl:Class ;
                    rdfs:subClassOf odrl:Asset ,
                                    [ rdf:type owl:Restriction ;
                                      owl:onProperty odrl:partOf ;
                                      owl:someValuesFrom :SystemGeneralDescription
                                    ] ;
                    rdfs:label "Instructions for Use"@en ;
                    skos:definition "‘instructions for use’ or ‘instructions of use’ means the information provided by the provider to inform the user of in particular an AI system’s intended purpose and proper use, inclusive of the specific geographical, behavioural or functional setting within which the high-risk AI system is intended to be used."@en ;
                    skos:note "Article 3 (15)" ;
                    odrl:source "https://eur-lex.europa.eu/legal-content/EN/TXT/HTML/?uri=CELEX:52021PC0206&from=EN" .


###  https://w3id.org/stav#IntendedBenefitsOverPreviouslyExistingProcess
:IntendedBenefitsOverPreviouslyExistingProcess rdf:type owl:Class ;
                                               rdfs:subClassOf odrl:Asset ;
                                               rdfs:comment """\"intended benefits\"
Sec. 4. (a) (1) (C)
S. 2892: Algorithmic Accountability Act of 2023
https://www.govtrack.us/congress/bills/118/s2892/text/is#link=4_a_1_C

\"benefits\"
Sec. 203. (a) (2) (D)
S. 3312: Artificial Intelligence Research, Innovation, and Accountability Act of 2023
https://www.govtrack.us/congress/bills/118/s3312/text/is#link=II_203_a_2_D&nearest=id18d5fa12eea943a799b7e1075a62e1bf"""@en ;
                                               rdfs:label "Intended Benefits Over Previously Existing Process"@en ;
                                               skos:definition "Intended benefits of and need for the new process."@en .


###  https://w3id.org/stav#IntendedHardwareDescription
:IntendedHardwareDescription rdf:type owl:Class ;
                             rdfs:subClassOf odrl:Asset ;
                             rdfs:comment "Annex IV (1) (e) EU AI Act"@en ;
                             rdfs:label "Intended Hardware Description"@en ;
                             skos:definition "The description of hardware on which the AI system is intended to run."@en .


###  https://w3id.org/stav#IntendedPurposes
:IntendedPurposes rdf:type owl:Class ;
                  rdfs:subClassOf odrl:Asset ;
                  rdfs:comment """\"intended purpose\"
EU AI Act
Annex IV (1) (b)
Annex VIII Section C (4)
Annex VIII Section A (5)
Annex VIIIa (3)

\"purpose\"
Sec. 203. (a) (2) (A)
S.3312 - Artificial Intelligence Research, Innovation, and Accountability Act of 2023
https://www.govtrack.us/congress/bills/118/s3312/text/is#link=II_203_a_2_A&nearest=id228689ffe9534563b8ce28c344358201

\"intended purpose\"
Sec. 4 (a) (1) (D)
S. 2892: Algorithmic Accountability Act of 2023
https://www.govtrack.us/congress/bills/118/s2892/text/is#link=4_a_1_D_~T1&nearest=idCD671E7BFB0C45779B5E8802FF584BB4

\"intended purpose\"
Sec. 5. (1) (C)
S. 2892: Algorithmic Accountability Act of 2023
https://www.govtrack.us/congress/bills/118/s2892/text/is#link=5_1_C_~T1&nearest=idf074706698514621a84859fffa6b6fed"""@en ;
                  rdfs:label "Intended Purposes"@en .


###  https://w3id.org/stav#Log
:Log rdf:type owl:Class ;
     rdfs:subClassOf odrl:Asset ;
     rdfs:label "Log"@en ;
     skos:definition "Automatic recording of events while the high-risk AI systems is operating. Those logging capabilities shall conform to recognised standards or common specifications. The logging capabilities shall ensure a level of traceability of the AI system’s functioning throughout its lifecycle that is appropriate to the intended purpose of the system."@en ;
     skos:note "Article 12" ;
     odrl:source "https://eur-lex.europa.eu/legal-content/EN/TXT/HTML/?uri=CELEX:52021PC0206&from=EN" .


###  https://w3id.org/stav#MakingAvailableOnTheMarket
:MakingAvailableOnTheMarket rdf:type owl:Class ;
                            rdfs:subClassOf odrl:Action ;
                            rdfs:label "making available on the market"@en ;
                            skos:definition "‘making available on the market’ means any supply of an AI system for distribution or use on the Union market in the course of a commercial activity, whether in return for payment or free of charge."@en ;
                            skos:note "Article 3 (10)" ;
                            odrl:source "https://eur-lex.europa.eu/legal-content/EN/TXT/HTML/?uri=CELEX:52021PC0206&from=EN" .


###  https://w3id.org/stav#MarketSurveillenceAuthority
:MarketSurveillenceAuthority rdf:type owl:Class ;
                             rdfs:subClassOf odrl:Party ;
                             rdfs:label "Market Surveillence Authority"@en ;
                             skos:note "Article 3 (26)" ;
                             odrl:source "https://eur-lex.europa.eu/legal-content/EN/TXT/HTML/?uri=CELEX:52021PC0206&from=EN" .


###  https://w3id.org/stav#PlacingOnTheMarket
:PlacingOnTheMarket rdf:type owl:Class ;
                    rdfs:subClassOf odrl:Action ;
                    rdfs:label "placing on the market"@en ;
                    skos:definition "‘placing on the market’ means the first making available of an AI system on the Union market."@en ;
                    skos:note "Article 3 (9)" ;
                    odrl:source "https://eur-lex.europa.eu/legal-content/EN/TXT/HTML/?uri=CELEX:52021PC0206&from=EN" .


###  https://w3id.org/stav#PostMarketEvaluationSystemDescription
:PostMarketEvaluationSystemDescription rdf:type owl:Class ;
                                       rdfs:subClassOf odrl:Asset ;
                                       rdfs:comment "Annex IV (8) EU AI Act"@en ;
                                       rdfs:label "Post-Market Evaluation System Description"@en .


###  https://w3id.org/stav#PreviouslyExistingProcessEvaluationDocumentation
:PreviouslyExistingProcessEvaluationDocumentation rdf:type owl:Class ;
                                                  rdfs:subClassOf odrl:AssetCollection ;
                                                  rdfs:comment """Sec. 4. (a) (1)
S. 2892: Algorithmic Accountability Act of 2023
https://www.govtrack.us/congress/bills/118/s2892/text/is#link=4_a_1

\"In the case of a new augmented critical decision process, evaluate any previously existing critical decision-making process used for the same critical decision prior to the deployment of the new augmented critical decision process, along with any related documentation or information, such as—

(A) a description of the baseline process being enhanced or replaced by the augmented critical decision process;

(B) any known harm, shortcoming, failure case, or material negative impact on consumers of the previously existing process used to make the critical decision;

(C) the intended benefits of and need for the augmented critical decision process; and

(D) the intended purpose of the automated decision system or augmented critical decision process.\""""@en ;
                                                  rdfs:label "Previously Existing Process Evaluation Documentation"@en ;
                                                  skos:definition "Any related documentation or information about previously existing process being enhanced or replaced by the new process. This also includes information about the new process for the comparison purpose with the previously existing process."@en .


###  https://w3id.org/stav#PreviouslyExistingProcessKnownNegativeImpactInformation
:PreviouslyExistingProcessKnownNegativeImpactInformation rdf:type owl:Class ;
                                                         rdfs:subClassOf odrl:Asset ;
                                                         rdfs:label "Previously Existing Process Known Negative Impact Information"@en ;
                                                         skos:definition "Any known harm, shortcoming, failure case, or material negative impact on consumers of the previously existing process used to make a decision."@en .


###  https://w3id.org/stav#PrivacyRisksAndPrivacyMeasuresEvaluationDocumentation
:PrivacyRisksAndPrivacyMeasuresEvaluationDocumentation rdf:type owl:Class ;
                                                       rdfs:subClassOf odrl:AssetCollection ;
                                                       rdfs:label "Privacy Risks and Privacy Measures Evaluation Documentation"@en .


###  https://w3id.org/stav#ProductServiceDescription
:ProductServiceDescription rdf:type owl:Class ;
                           rdfs:subClassOf odrl:Asset ;
                           rdfs:comment "Annex IV (1) (d) EU AI Act"@en ;
                           rdfs:label "Product Service Descriptipn"@en ;
                           skos:definition """The description of the form in which the AI system is placed on the market or put into service.

One AI system can has more than one form of product or service."""@en .


###  https://w3id.org/stav#ProductVisualImage
:ProductVisualImage rdf:type owl:Class ;
                    rdfs:subClassOf odrl:Asset ;
                    rdfs:comment """Annex IV (1) (f) EU AI Act

(f) where the AI system is a component of products, photographs or illustrations showing external features, marking and internal layout of those products;"""@en ;
                    rdfs:label "Product Visual Image"@en ;
                    skos:definition "A photograph or an illustration showing external features, marking, and internal layout of a product that the AI system is part of."@en .


###  https://w3id.org/stav#PuttingIntoService
:PuttingIntoService rdf:type owl:Class ;
                    rdfs:subClassOf odrl:Action ;
                    rdfs:label "putting into service"@en ;
                    skos:definition "‘putting into service’ means the supply of an AI system for first use directly to the user or for own use on the Union market for its intended purpose."@en ;
                    skos:note "Article 3 (11)"@en ;
                    odrl:source "https://eur-lex.europa.eu/legal-content/EN/TXT/HTML/?uri=CELEX:52021PC0206&from=EN" .


###  https://w3id.org/stav#QualityManagementSystemDocumentationObligation
:QualityManagementSystemDocumentationObligation rdf:type owl:Class ;
                                                rdfs:subClassOf stap:InformationCreationObligation ;
                                                rdfs:label "Quality Management System Documentation Obligation"@en ;
                                                skos:definition "A quality management system ensures compliance of an AI system. A quality management system documentation shall be in the form of written policies, procedures and instructions. It shall include a strategy for regulatory compliance; techniques, procedures and systematic actions to be used for the design, development, and examination of the AI system, etc."@en .


###  https://w3id.org/stav#RealWorldConditionsTestingPlan
:RealWorldConditionsTestingPlan rdf:type owl:Class ;
                                rdfs:subClassOf odrl:Asset ;
                                rdfs:comment "A summary of the main characteristics of the plan for testing in real world conditions."@en ;
                                rdfs:label "Real World Conditions Testing Plan"@en ;
                                skos:note "EU AI Act Annex VIIIa (4)"@en .


###  https://w3id.org/stav#RealWorldConditionsTestingSuspensionOrTerminationInformation
:RealWorldConditionsTestingSuspensionOrTerminationInformation rdf:type owl:Class ;
                                                              rdfs:subClassOf odrl:Asset ;
                                                              rdfs:comment "Information on the suspension or termination of the testing in real world conditions."@en ;
                                                              rdfs:label "Real World Conditions Testing Suspension Or Termination Information"@en ;
                                                              skos:note "EU AI Act Annex VIIIa (5)"@en .


###  https://w3id.org/stav#RealWorldConditionsTestingUser
:RealWorldConditionsTestingUser rdf:type owl:Class ;
                                rdfs:subClassOf odrl:Party ;
                                rdfs:comment "users involved in the testing in real world conditions."@en ;
                                rdfs:label "Real World Conditions Testing User"@en ;
                                skos:note "EU AI Act Annex VIIIa (2)"@en .


###  https://w3id.org/stav#RegisterationObligation
:RegisterationObligation rdf:type owl:Class ;
                         rdfs:subClassOf stap:InformationSubmissionObligation ;
                         rdfs:label "Registeration Obligation"@en ;
                         skos:definition "A registration to a database containing information about AI systems."@en .


###  https://w3id.org/stav#RiskManagementSystemDescription
:RiskManagementSystemDescription rdf:type owl:Class ;
                                 rdfs:subClassOf odrl:Asset ;
                                 rdfs:label "Risk Management System Description"@en .


###  https://w3id.org/stav#SoftwareDependencies
:SoftwareDependencies rdf:type owl:Class ;
                      rdfs:subClassOf odrl:Asset ;
                      rdfs:comment """Annex IV (1) (c) EU AI Act

This is the area that Software Bill of Materials can help a lot.

\"versions of relevant software or firmware\" can taken from software metadata that package manager already have.

The \"any requirement related to version update\" could be a narrative one and need further clarification."""@en ;
                      rdfs:label "Software Dependencies"@en ;
                      skos:definition "The versions of relevant software or firmware and any requirement related to version update."@en .


###  https://w3id.org/stav#SystemDetailedDescription
:SystemDetailedDescription rdf:type owl:Class ;
                           rdfs:subClassOf odrl:AssetCollection ;
                           rdfs:label "System Detailed Description"@en .


###  https://w3id.org/stav#SystemEvaluationDocumentation
:SystemEvaluationDocumentation rdf:type owl:Class ;
                               rdfs:subClassOf odrl:AssetCollection ;
                               rdfs:label "System Evaluation Documentation" .


###  https://w3id.org/stav#SystemGeneralDescription
:SystemGeneralDescription rdf:type owl:Class ;
                          rdfs:subClassOf odrl:AssetCollection ;
                          rdfs:comment """Similar to what defined in Annex IV (1) of EU AI Act,
as part of the Technical Documentation referred to in Article 11 (1)"""@en ;
                          rdfs:label "System General Description"@en ;
                          skos:definition "A general description of the AI system."@en .


###  https://w3id.org/stav#TechnicalDocumentation
:TechnicalDocumentation rdf:type owl:Class ;
                        rdfs:subClassOf odrl:AssetCollection ;
                        rdfs:comment """Similar to \"Transparency Report\"
as defined in Sec. 203. (a) (2) of
S.3312 - Artificial Intelligence Research, Innovation, and Accountability Act of 2023
https://www.govtrack.us/congress/bills/118/s3312/text/is#link=II_203_a_2"""@en ;
                        rdfs:label "Technical Documentation"@en ;
                        skos:definition "The technical documentation shall be drawn up in such a way to demonstrate that the high-risk AI system complies with the requirements set out in Title III Chapter 2 and provide national competent authorities and notified bodies with all the necessary information to assess the compliance of the AI system with those requirements. It shall contain, at a minimum, the elements set out in Annex IV."@en ;
                        skos:note "Article 11" ;
                        odrl:source "https://eur-lex.europa.eu/legal-content/EN/TXT/HTML/?uri=CELEX:52021PC0206&from=EN" .


###  https://w3id.org/stav#TechnicalDocumentationObligation
:TechnicalDocumentationObligation rdf:type owl:Class ;
                                  rdfs:subClassOf stap:InformationCreationObligation ;
                                  rdfs:label "Technical Documentation Obligation"@en ;
                                  skos:definition "The technical documentation of an AI system contains information including its intended purpose and limitations, risk management process, data governance, and instructions of use."@en .


###  Generated by the OWL API (version 4.5.26.2023-07-17T20:34:13Z) https://github.com/owlcs/owlapi
