<?xml version="1.0"?>
<rdf:RDF xmlns="https://w3id.org/stav#"
     xml:base="https://w3id.org/stav"
     xmlns:owl="http://www.w3.org/2002/07/owl#"
     xmlns:rdf="http://www.w3.org/1999/02/22-rdf-syntax-ns#"
     xmlns:xml="http://www.w3.org/XML/1998/namespace"
     xmlns:xsd="http://www.w3.org/2001/XMLSchema#"
     xmlns:odrl="http://www.w3.org/ns/odrl/2/"
     xmlns:rdfs="http://www.w3.org/2000/01/rdf-schema#"
     xmlns:skos="http://www.w3.org/2004/02/skos/core#"
     xmlns:terms="http://purl.org/dc/terms/">
    <owl:Ontology rdf:about="https://w3id.org/stav">
        <owl:versionIRI rdf:resource="https://w3id.org/stav/0.5"/>
        <owl:imports rdf:resource="http://spdx.org/rdf/terms/2.3"/>
        <owl:imports rdf:resource="https://w3id.org/stap/0.1"/>
        <terms:creator>Arthit Suriyawongkul</terms:creator>
        <terms:description xml:lang="en">STAV represents AI system accountability concepts and relations.</terms:description>
        <terms:issued>2024-01-14T18:30:00</terms:issued>
        <terms:license>https://creativecommons.org/licenses/by/4.0/</terms:license>
        <terms:modified>2024-04-16T14:30:00</terms:modified>
        <terms:publisher>ADAPT Centre, Trinity College Dublin</terms:publisher>
        <terms:title>STAV</terms:title>
        <rdfs:label xml:lang="en">System Trustworthiness and Accountability Vocabulary</rdfs:label>
        <owl:versionInfo rdf:datatype="http://www.w3.org/2001/XMLSchema#decimal">0.5</owl:versionInfo>
    </owl:Ontology>
    


    <!-- 
    ///////////////////////////////////////////////////////////////////////////////////////
    //
    // Annotation properties
    //
    ///////////////////////////////////////////////////////////////////////////////////////
     -->


    


    <!-- http://purl.org/dc/terms/creator -->


    <owl:AnnotationProperty rdf:about="http://purl.org/dc/terms/creator"/>
    


    <!-- http://purl.org/dc/terms/description -->


    <owl:AnnotationProperty rdf:about="http://purl.org/dc/terms/description"/>
    


    <!-- http://purl.org/dc/terms/issued -->


    <owl:AnnotationProperty rdf:about="http://purl.org/dc/terms/issued"/>
    


    <!-- http://purl.org/dc/terms/license -->


    <owl:AnnotationProperty rdf:about="http://purl.org/dc/terms/license"/>
    


    <!-- http://purl.org/dc/terms/modified -->


    <owl:AnnotationProperty rdf:about="http://purl.org/dc/terms/modified"/>
    


    <!-- http://purl.org/dc/terms/publisher -->


    <owl:AnnotationProperty rdf:about="http://purl.org/dc/terms/publisher"/>
    


    <!-- http://purl.org/dc/terms/title -->


    <owl:AnnotationProperty rdf:about="http://purl.org/dc/terms/title"/>
    


    <!-- http://www.w3.org/2004/02/skos/core#definition -->


    <owl:AnnotationProperty rdf:about="http://www.w3.org/2004/02/skos/core#definition"/>
    


    <!-- http://www.w3.org/2004/02/skos/core#note -->


    <owl:AnnotationProperty rdf:about="http://www.w3.org/2004/02/skos/core#note"/>
    


    <!-- http://www.w3.org/ns/odrl/2/source -->


    <owl:AnnotationProperty rdf:about="http://www.w3.org/ns/odrl/2/source"/>
    


    <!-- 
    ///////////////////////////////////////////////////////////////////////////////////////
    //
    // Datatypes
    //
    ///////////////////////////////////////////////////////////////////////////////////////
     -->


    


    <!-- https://w3id.org/stav#AISystemStatusType -->


    <rdfs:Datatype rdf:about="https://w3id.org/stav#AISystemStatusType">
        <owl:equivalentClass>
            <rdfs:Datatype>
                <owl:oneOf>
                    <rdf:Description>
                        <rdf:type rdf:resource="http://www.w3.org/1999/02/22-rdf-syntax-ns#List"/>
                        <rdf:first>In service</rdf:first>
                        <rdf:rest>
                            <rdf:Description>
                                <rdf:type rdf:resource="http://www.w3.org/1999/02/22-rdf-syntax-ns#List"/>
                                <rdf:first>No longer placed on the market/in service</rdf:first>
                                <rdf:rest>
                                    <rdf:Description>
                                        <rdf:type rdf:resource="http://www.w3.org/1999/02/22-rdf-syntax-ns#List"/>
                                        <rdf:first>On the market</rdf:first>
                                        <rdf:rest>
                                            <rdf:Description>
                                                <rdf:type rdf:resource="http://www.w3.org/1999/02/22-rdf-syntax-ns#List"/>
                                                <rdf:first>Recalled</rdf:first>
                                                <rdf:rest rdf:resource="http://www.w3.org/1999/02/22-rdf-syntax-ns#nil"/>
                                            </rdf:Description>
                                        </rdf:rest>
                                    </rdf:Description>
                                </rdf:rest>
                            </rdf:Description>
                        </rdf:rest>
                    </rdf:Description>
                </owl:oneOf>
            </rdfs:Datatype>
        </owl:equivalentClass>
    </rdfs:Datatype>
    


    <!-- 
    ///////////////////////////////////////////////////////////////////////////////////////
    //
    // Object Properties
    //
    ///////////////////////////////////////////////////////////////////////////////////////
     -->


    


    <!-- http://www.w3.org/ns/odrl/2/duty -->


    <owl:ObjectProperty rdf:about="http://www.w3.org/ns/odrl/2/duty"/>
    


    <!-- http://www.w3.org/ns/odrl/2/partOf -->


    <owl:ObjectProperty rdf:about="http://www.w3.org/ns/odrl/2/partOf"/>
    


    <!-- https://w3id.org/stav#hasAddress -->


    <owl:ObjectProperty rdf:about="https://w3id.org/stav#hasAddress">
        <rdfs:subPropertyOf rdf:resource="http://www.w3.org/2002/07/owl#topObjectProperty"/>
        <rdfs:domain rdf:resource="https://w3id.org/stav#AIDeployer"/>
        <rdfs:domain rdf:resource="https://w3id.org/stav#AIProvider"/>
    </owl:ObjectProperty>
    


    <!-- https://w3id.org/stav#hasContactDetails -->


    <owl:ObjectProperty rdf:about="https://w3id.org/stav#hasContactDetails">
        <rdfs:subPropertyOf rdf:resource="http://www.w3.org/2002/07/owl#topObjectProperty"/>
        <rdfs:domain rdf:resource="https://w3id.org/stav#AIDeployer"/>
        <rdfs:domain rdf:resource="https://w3id.org/stav#AIProvider"/>
    </owl:ObjectProperty>
    


    <!-- https://w3id.org/stav#hasName -->


    <owl:ObjectProperty rdf:about="https://w3id.org/stav#hasName">
        <rdfs:domain rdf:resource="https://w3id.org/stav#AIDeployer"/>
        <rdfs:domain rdf:resource="https://w3id.org/stav#AIProvider"/>
        <rdfs:domain rdf:resource="https://w3id.org/stav#AISystem"/>
        <rdfs:domain rdf:resource="https://w3id.org/stav#AuthorisedRepresentative"/>
        <rdfs:domain rdf:resource="https://w3id.org/stav#InformationSubmissionRepresentative"/>
        <rdfs:domain rdf:resource="https://w3id.org/stav#MarketSurveillenceAuthority"/>
    </owl:ObjectProperty>
    


    <!-- https://w3id.org/stav#onBehalfOf -->


    <owl:ObjectProperty rdf:about="https://w3id.org/stav#onBehalfOf">
        <rdfs:subPropertyOf rdf:resource="http://www.w3.org/2002/07/owl#topObjectProperty"/>
    </owl:ObjectProperty>
    


    <!-- 
    ///////////////////////////////////////////////////////////////////////////////////////
    //
    // Classes
    //
    ///////////////////////////////////////////////////////////////////////////////////////
     -->


    


    <!-- http://www.w3.org/ns/odrl/2/Action -->


    <owl:Class rdf:about="http://www.w3.org/ns/odrl/2/Action"/>
    


    <!-- http://www.w3.org/ns/odrl/2/Asset -->


    <owl:Class rdf:about="http://www.w3.org/ns/odrl/2/Asset"/>
    


    <!-- http://www.w3.org/ns/odrl/2/AssetCollection -->


    <owl:Class rdf:about="http://www.w3.org/ns/odrl/2/AssetCollection"/>
    


    <!-- http://www.w3.org/ns/odrl/2/Party -->


    <owl:Class rdf:about="http://www.w3.org/ns/odrl/2/Party"/>
    


    <!-- https://w3id.org/stap#InformationCreationObligation -->


    <owl:Class rdf:about="https://w3id.org/stap#InformationCreationObligation"/>
    


    <!-- https://w3id.org/stap#InformationSubmissionObligation -->


    <owl:Class rdf:about="https://w3id.org/stap#InformationSubmissionObligation"/>
    


    <!-- https://w3id.org/stav#AIDeployer -->


    <owl:Class rdf:about="https://w3id.org/stav#AIDeployer">
        <rdfs:subClassOf rdf:resource="http://www.w3.org/ns/odrl/2/Party"/>
        <rdfs:label xml:lang="en">AI Deployer</rdfs:label>
        <skos:note>Article 3 (4)</skos:note>
        <odrl:source>https://eur-lex.europa.eu/legal-content/EN/TXT/HTML/?uri=CELEX:52021PC0206&amp;from=EN</odrl:source>
    </owl:Class>
    


    <!-- https://w3id.org/stav#AIProvider -->


    <owl:Class rdf:about="https://w3id.org/stav#AIProvider">
        <rdfs:subClassOf rdf:resource="http://www.w3.org/ns/odrl/2/Party"/>
        <rdfs:label xml:lang="en">AI Provider</rdfs:label>
        <skos:note>Article 3 (2)</skos:note>
        <odrl:source>https://eur-lex.europa.eu/legal-content/EN/TXT/HTML/?uri=CELEX:52021PC0206&amp;from=EN</odrl:source>
    </owl:Class>
    


    <!-- https://w3id.org/stav#AISystem -->


    <owl:Class rdf:about="https://w3id.org/stav#AISystem">
        <rdfs:subClassOf rdf:resource="http://www.w3.org/ns/odrl/2/Asset"/>
        <rdfs:label xml:lang="en">AI System</rdfs:label>
    </owl:Class>
    


    <!-- https://w3id.org/stav#AISystemStatus -->


    <owl:Class rdf:about="https://w3id.org/stav#AISystemStatus">
        <rdfs:subClassOf rdf:resource="http://www.w3.org/ns/odrl/2/Asset"/>
    </owl:Class>
    


    <!-- https://w3id.org/stav#AppliedStandards -->


    <owl:Class rdf:about="https://w3id.org/stav#AppliedStandards">
        <rdfs:subClassOf rdf:resource="http://www.w3.org/ns/odrl/2/Asset"/>
        <rdfs:comment xml:lang="en">Annex IV (6)</rdfs:comment>
        <rdfs:label xml:lang="en">Applied Standards</rdfs:label>
    </owl:Class>
    


    <!-- https://w3id.org/stav#AuthorisedRepresentative -->


    <owl:Class rdf:about="https://w3id.org/stav#AuthorisedRepresentative">
        <rdfs:subClassOf rdf:resource="http://www.w3.org/ns/odrl/2/Party"/>
        <rdfs:label xml:lang="en">Authorised Representative</rdfs:label>
        <skos:note xml:lang="en">EU AI Act Annex VIII Section C (2)</skos:note>
    </owl:Class>
    


    <!-- https://w3id.org/stav#BaselineProcessDescription -->


    <owl:Class rdf:about="https://w3id.org/stav#BaselineProcessDescription">
        <rdfs:subClassOf rdf:resource="http://www.w3.org/ns/odrl/2/Asset"/>
        <rdfs:comment xml:lang="en">Sec. 4. (a) (1) (A)
S. 2892: Algorithmic Accountability Act of 2023
https://www.govtrack.us/congress/bills/118/s2892/text/is#link=4_a_1_A</rdfs:comment>
        <rdfs:label xml:lang="en">Baseline Process Description</rdfs:label>
        <skos:definition xml:lang="en">Desciption of a previously existing decision-making process prior to the deployment of an AI/augmented decision process.</skos:definition>
    </owl:Class>
    


    <!-- https://w3id.org/stav#BeingNotHighRiskCriteria -->


    <owl:Class rdf:about="https://w3id.org/stav#BeingNotHighRiskCriteria">
        <rdfs:subClassOf rdf:resource="http://www.w3.org/ns/odrl/2/Asset"/>
        <rdfs:comment xml:lang="en">Based on which criterion or criteria provided in Article 6(2a) the AI system is considered as not high-risk</rdfs:comment>
        <rdfs:label xml:lang="en">Being Not High-Risk Criteria</rdfs:label>
        <skos:note xml:lang="en">EU AI Act Annex VIII Section C (5)</skos:note>
    </owl:Class>
    


    <!-- https://w3id.org/stav#BeingNotHighRiskGrounds -->


    <owl:Class rdf:about="https://w3id.org/stav#BeingNotHighRiskGrounds">
        <rdfs:subClassOf rdf:resource="http://www.w3.org/ns/odrl/2/Asset"/>
        <rdfs:comment xml:lang="en">Short summary of the grounds for considering the AI system as not high-risk in application of the procedure under Article 6(2a)</rdfs:comment>
        <rdfs:label xml:lang="en">Being Not High-Risk Grounds</rdfs:label>
        <skos:note xml:lang="en">EU AI Act Annex VIII Section C (6)</skos:note>
    </owl:Class>
    


    <!-- https://w3id.org/stav#ComponentsAndFunctionsSupportedDescription -->


    <owl:Class rdf:about="https://w3id.org/stav#ComponentsAndFunctionsSupportedDescription">
        <rdfs:subClassOf rdf:resource="http://www.w3.org/ns/odrl/2/Asset"/>
        <rdfs:comment xml:lang="en">Description of the components and functions supported through this AI system</rdfs:comment>
        <rdfs:label xml:lang="en">Components And Functions Supported Description</rdfs:label>
        <skos:note xml:lang="en">EU AI Act Annex VIII Section A (5)</skos:note>
    </owl:Class>
    


    <!-- https://w3id.org/stav#ConformityDeclaration -->


    <owl:Class rdf:about="https://w3id.org/stav#ConformityDeclaration">
        <rdfs:subClassOf rdf:resource="http://www.w3.org/ns/odrl/2/Asset"/>
        <rdfs:comment xml:lang="en">Annex IV (7) EU AI Act

Can a text or an URL</rdfs:comment>
        <rdfs:label xml:lang="en">Conformity Declaration</rdfs:label>
    </owl:Class>
    


    <!-- https://w3id.org/stav#CurrentAndPotentialFutureImpacts -->


    <owl:Class rdf:about="https://w3id.org/stav#CurrentAndPotentialFutureImpacts">
        <rdfs:subClassOf rdf:resource="http://www.w3.org/ns/odrl/2/Asset"/>
        <rdfs:label xml:lang="en">Current and Potential Future Impacts</rdfs:label>
        <skos:definition xml:lang="en">Assessment and documentation of the current and potential future or downstream positive and negative impacts of a system or process.</skos:definition>
    </owl:Class>
    


    <!-- https://w3id.org/stav#DataMinimizationPractices -->


    <owl:Class rdf:about="https://w3id.org/stav#DataMinimizationPractices">
        <rdfs:subClassOf rdf:resource="http://www.w3.org/ns/odrl/2/Asset"/>
        <rdfs:label xml:lang="en">Data Minimization Practices</rdfs:label>
        <skos:definition xml:lang="en">Assessment and documentation of the data minimization practices of a system or process and the duration for which the relevant identifying information and any resulting critical decision is stored.</skos:definition>
    </owl:Class>
    


    <!-- https://w3id.org/stav#DataProtectionImpactAssessmentDocumentation -->


    <owl:Class rdf:about="https://w3id.org/stav#DataProtectionImpactAssessmentDocumentation">
        <rdfs:subClassOf rdf:resource="https://w3id.org/stav#ImpactAssessmentDocumentation"/>
        <rdfs:comment xml:lang="en">A summary of the data protection impact assessment carried out in accordance with Article 35 of Regulation (EU) 2016/679 or Article 27 of Directive (EU) 2016/680 as specified in paragraph 6 of Article 29 of this Regulation, where applicable.</rdfs:comment>
        <rdfs:label xml:lang="en">Data Protection Impact Assessment Documentation</rdfs:label>
        <skos:note xml:lang="en">EU AI Act Annex VIII Section B (7)</skos:note>
    </owl:Class>
    


    <!-- https://w3id.org/stav#DeploymentContext -->


    <owl:Class rdf:about="https://w3id.org/stav#DeploymentContext">
        <rdfs:subClassOf rdf:resource="http://www.w3.org/ns/odrl/2/Asset"/>
        <rdfs:comment xml:lang="en">Sec. 203. (a) (2) (C)
S. 3312: Artificial Intelligence Research, Innovation, and Accountability Act of 2023
https://www.govtrack.us/congress/bills/118/s3312/text/is#link=II_203_a_2_C&amp;nearest=id07706866948d4dc59792b34859a3afdf</rdfs:comment>
        <rdfs:label xml:lang="en">Deployment Context</rdfs:label>
    </owl:Class>
    


    <!-- https://w3id.org/stav#ExternalInteractionDescription -->


    <owl:Class rdf:about="https://w3id.org/stav#ExternalInteractionDescription">
        <rdfs:subClassOf rdf:resource="http://www.w3.org/ns/odrl/2/Asset"/>
        <rdfs:comment>EU AI Act Annex IV (1) (b)</rdfs:comment>
        <rdfs:label xml:lang="en">External Interaction Description</rdfs:label>
        <skos:definition xml:lang="en">How the AI system interacts or can be used to interact with hardware or software that is not part of the AI system itself, where applicable.</skos:definition>
    </owl:Class>
    


    <!-- https://w3id.org/stav#FundamentalRightsImpactAssessmentDocumentation -->


    <owl:Class rdf:about="https://w3id.org/stav#FundamentalRightsImpactAssessmentDocumentation">
        <rdfs:subClassOf rdf:resource="https://w3id.org/stav#ImpactAssessmentDocumentation"/>
        <rdfs:comment xml:lang="en">A summary of the findings of the fundamental rights impact assessment conducted in accordance with Article 29a.</rdfs:comment>
        <rdfs:label xml:lang="en">Fundamental Rights Impact Assessment Documentation</rdfs:label>
        <skos:note xml:lang="en">EU AI Act Annex VIII Section B (5)</skos:note>
    </owl:Class>
    


    <!-- https://w3id.org/stav#ImpactAssessmentDocumentation -->


    <owl:Class rdf:about="https://w3id.org/stav#ImpactAssessmentDocumentation">
        <rdfs:subClassOf rdf:resource="http://www.w3.org/ns/odrl/2/AssetCollection"/>
        <rdfs:comment xml:lang="en">S. 2892: Algorithmic Accountability Act of 2023
Defined in Sec. 2. (12)
https://www.govtrack.us/congress/bills/118/s2892/text/is#link=2_12
and detailed in Sec. 4. (a)
https://www.govtrack.us/congress/bills/118/s2892/text/is#link=4_a

S. 3312: Artificial Intelligence Research, Innovation, and Accountability Act of 2023
Title II Sec. 206. (b)
https://www.govtrack.us/congress/bills/118/s3312/text/is#link=II_206_b</rdfs:comment>
        <rdfs:label>Impact Assessment Documentation</rdfs:label>
    </owl:Class>
    


    <!-- https://w3id.org/stav#InformationSecurityMeasures -->


    <owl:Class rdf:about="https://w3id.org/stav#InformationSecurityMeasures">
        <rdfs:subClassOf rdf:resource="http://www.w3.org/ns/odrl/2/Asset"/>
        <rdfs:label xml:lang="en">Information Security Measures</rdfs:label>
        <skos:definition xml:lang="en">Assessment of information security measures with respect to a system or process.</skos:definition>
    </owl:Class>
    


    <!-- https://w3id.org/stav#InformationSubmissionRepresentative -->


    <owl:Class rdf:about="https://w3id.org/stav#InformationSubmissionRepresentative">
        <rdfs:subClassOf rdf:resource="http://www.w3.org/ns/odrl/2/Party"/>
        <rdfs:label xml:lang="en">Information Submission Representative</rdfs:label>
        <skos:note xml:lang="en">EU AI Act Annex VIII Section C (1)</skos:note>
    </owl:Class>
    


    <!-- https://w3id.org/stav#InformationUsedBySystemDescription -->


    <owl:Class rdf:about="https://w3id.org/stav#InformationUsedBySystemDescription">
        <rdfs:subClassOf rdf:resource="http://www.w3.org/ns/odrl/2/Asset"/>
        <rdfs:comment xml:lang="en">A basic and concise description of the information used by the system (data, inputs) and its operating logic</rdfs:comment>
        <rdfs:label xml:lang="en">Information Used By the System Description</rdfs:label>
        <skos:note xml:lang="en">EU AI Act Annex VIII Section A (5a)</skos:note>
    </owl:Class>
    


    <!-- https://w3id.org/stav#InstallationInstructions -->


    <owl:Class rdf:about="https://w3id.org/stav#InstallationInstructions">
        <rdfs:subClassOf rdf:resource="http://www.w3.org/ns/odrl/2/Asset"/>
        <rdfs:subClassOf>
            <owl:Restriction>
                <owl:onProperty rdf:resource="http://www.w3.org/ns/odrl/2/partOf"/>
                <owl:someValuesFrom rdf:resource="https://w3id.org/stav#SystemGeneralDescription"/>
            </owl:Restriction>
        </rdfs:subClassOf>
        <rdfs:label xml:lang="en">Installation Instructions</rdfs:label>
    </owl:Class>
    


    <!-- https://w3id.org/stav#InstructionsForUse -->


    <owl:Class rdf:about="https://w3id.org/stav#InstructionsForUse">
        <rdfs:subClassOf rdf:resource="http://www.w3.org/ns/odrl/2/Asset"/>
        <rdfs:subClassOf>
            <owl:Restriction>
                <owl:onProperty rdf:resource="http://www.w3.org/ns/odrl/2/partOf"/>
                <owl:someValuesFrom rdf:resource="https://w3id.org/stav#SystemGeneralDescription"/>
            </owl:Restriction>
        </rdfs:subClassOf>
        <rdfs:label xml:lang="en">Instructions for Use</rdfs:label>
        <skos:definition xml:lang="en">‘instructions for use’ or ‘instructions of use’ means the information provided by the provider to inform the user of in particular an AI system’s intended purpose and proper use, inclusive of the specific geographical, behavioural or functional setting within which the high-risk AI system is intended to be used.</skos:definition>
        <skos:note>Article 3 (15)</skos:note>
        <odrl:source>https://eur-lex.europa.eu/legal-content/EN/TXT/HTML/?uri=CELEX:52021PC0206&amp;from=EN</odrl:source>
    </owl:Class>
    


    <!-- https://w3id.org/stav#IntendedBenefitsOverPreviouslyExistingProcess -->


    <owl:Class rdf:about="https://w3id.org/stav#IntendedBenefitsOverPreviouslyExistingProcess">
        <rdfs:subClassOf rdf:resource="http://www.w3.org/ns/odrl/2/Asset"/>
        <rdfs:comment xml:lang="en">&quot;intended benefits&quot;
Sec. 4. (a) (1) (C)
S. 2892: Algorithmic Accountability Act of 2023
https://www.govtrack.us/congress/bills/118/s2892/text/is#link=4_a_1_C

&quot;benefits&quot;
Sec. 203. (a) (2) (D)
S. 3312: Artificial Intelligence Research, Innovation, and Accountability Act of 2023
https://www.govtrack.us/congress/bills/118/s3312/text/is#link=II_203_a_2_D&amp;nearest=id18d5fa12eea943a799b7e1075a62e1bf</rdfs:comment>
        <rdfs:label xml:lang="en">Intended Benefits Over Previously Existing Process</rdfs:label>
        <skos:definition xml:lang="en">Intended benefits of and need for the new process.</skos:definition>
    </owl:Class>
    


    <!-- https://w3id.org/stav#IntendedHardwareDescription -->


    <owl:Class rdf:about="https://w3id.org/stav#IntendedHardwareDescription">
        <rdfs:subClassOf rdf:resource="http://www.w3.org/ns/odrl/2/Asset"/>
        <rdfs:comment xml:lang="en">Annex IV (1) (e) EU AI Act</rdfs:comment>
        <rdfs:label xml:lang="en">Intended Hardware Description</rdfs:label>
        <skos:definition xml:lang="en">The description of hardware on which the AI system is intended to run.</skos:definition>
    </owl:Class>
    


    <!-- https://w3id.org/stav#IntendedPurposes -->


    <owl:Class rdf:about="https://w3id.org/stav#IntendedPurposes">
        <rdfs:subClassOf rdf:resource="http://www.w3.org/ns/odrl/2/Asset"/>
        <rdfs:comment xml:lang="en">&quot;intended purpose&quot;
EU AI Act
Annex IV (1) (b)
Annex VIII Section C (4)
Annex VIII Section A (5)
Annex VIIIa (3)

&quot;purpose&quot;
Sec. 203. (a) (2) (A)
S.3312 - Artificial Intelligence Research, Innovation, and Accountability Act of 2023
https://www.govtrack.us/congress/bills/118/s3312/text/is#link=II_203_a_2_A&amp;nearest=id228689ffe9534563b8ce28c344358201

&quot;intended purpose&quot;
Sec. 4 (a) (1) (D)
S. 2892: Algorithmic Accountability Act of 2023
https://www.govtrack.us/congress/bills/118/s2892/text/is#link=4_a_1_D_~T1&amp;nearest=idCD671E7BFB0C45779B5E8802FF584BB4

&quot;intended purpose&quot;
Sec. 5. (1) (C)
S. 2892: Algorithmic Accountability Act of 2023
https://www.govtrack.us/congress/bills/118/s2892/text/is#link=5_1_C_~T1&amp;nearest=idf074706698514621a84859fffa6b6fed</rdfs:comment>
        <rdfs:label xml:lang="en">Intended Purposes</rdfs:label>
    </owl:Class>
    


    <!-- https://w3id.org/stav#Log -->


    <owl:Class rdf:about="https://w3id.org/stav#Log">
        <rdfs:subClassOf rdf:resource="http://www.w3.org/ns/odrl/2/Asset"/>
        <rdfs:label xml:lang="en">Log</rdfs:label>
        <skos:definition xml:lang="en">Automatic recording of events while the high-risk AI systems is operating. Those logging capabilities shall conform to recognised standards or common specifications. The logging capabilities shall ensure a level of traceability of the AI system’s functioning throughout its lifecycle that is appropriate to the intended purpose of the system.</skos:definition>
        <skos:note>Article 12</skos:note>
        <odrl:source>https://eur-lex.europa.eu/legal-content/EN/TXT/HTML/?uri=CELEX:52021PC0206&amp;from=EN</odrl:source>
    </owl:Class>
    


    <!-- https://w3id.org/stav#MakingAvailableOnTheMarket -->


    <owl:Class rdf:about="https://w3id.org/stav#MakingAvailableOnTheMarket">
        <rdfs:subClassOf rdf:resource="http://www.w3.org/ns/odrl/2/Action"/>
        <rdfs:label xml:lang="en">making available on the market</rdfs:label>
        <skos:definition xml:lang="en">‘making available on the market’ means any supply of an AI system for distribution or use on the Union market in the course of a commercial activity, whether in return for payment or free of charge.</skos:definition>
        <skos:note>Article 3 (10)</skos:note>
        <odrl:source>https://eur-lex.europa.eu/legal-content/EN/TXT/HTML/?uri=CELEX:52021PC0206&amp;from=EN</odrl:source>
    </owl:Class>
    


    <!-- https://w3id.org/stav#MarketSurveillenceAuthority -->


    <owl:Class rdf:about="https://w3id.org/stav#MarketSurveillenceAuthority">
        <rdfs:subClassOf rdf:resource="http://www.w3.org/ns/odrl/2/Party"/>
        <rdfs:label xml:lang="en">Market Surveillence Authority</rdfs:label>
        <skos:note>Article 3 (26)</skos:note>
        <odrl:source>https://eur-lex.europa.eu/legal-content/EN/TXT/HTML/?uri=CELEX:52021PC0206&amp;from=EN</odrl:source>
    </owl:Class>
    


    <!-- https://w3id.org/stav#PlacingOnTheMarket -->


    <owl:Class rdf:about="https://w3id.org/stav#PlacingOnTheMarket">
        <rdfs:subClassOf rdf:resource="http://www.w3.org/ns/odrl/2/Action"/>
        <rdfs:label xml:lang="en">placing on the market</rdfs:label>
        <skos:definition xml:lang="en">‘placing on the market’ means the first making available of an AI system on the Union market.</skos:definition>
        <skos:note>Article 3 (9)</skos:note>
        <odrl:source>https://eur-lex.europa.eu/legal-content/EN/TXT/HTML/?uri=CELEX:52021PC0206&amp;from=EN</odrl:source>
    </owl:Class>
    


    <!-- https://w3id.org/stav#PostMarketEvaluationSystemDescription -->


    <owl:Class rdf:about="https://w3id.org/stav#PostMarketEvaluationSystemDescription">
        <rdfs:subClassOf rdf:resource="http://www.w3.org/ns/odrl/2/Asset"/>
        <rdfs:comment xml:lang="en">Annex IV (8) EU AI Act</rdfs:comment>
        <rdfs:label xml:lang="en">Post-Market Evaluation System Description</rdfs:label>
    </owl:Class>
    


    <!-- https://w3id.org/stav#PreviouslyExistingProcessEvaluationDocumentation -->


    <owl:Class rdf:about="https://w3id.org/stav#PreviouslyExistingProcessEvaluationDocumentation">
        <rdfs:subClassOf rdf:resource="http://www.w3.org/ns/odrl/2/AssetCollection"/>
        <rdfs:comment xml:lang="en">Sec. 4. (a) (1)
S. 2892: Algorithmic Accountability Act of 2023
https://www.govtrack.us/congress/bills/118/s2892/text/is#link=4_a_1

&quot;In the case of a new augmented critical decision process, evaluate any previously existing critical decision-making process used for the same critical decision prior to the deployment of the new augmented critical decision process, along with any related documentation or information, such as—

(A) a description of the baseline process being enhanced or replaced by the augmented critical decision process;

(B) any known harm, shortcoming, failure case, or material negative impact on consumers of the previously existing process used to make the critical decision;

(C) the intended benefits of and need for the augmented critical decision process; and

(D) the intended purpose of the automated decision system or augmented critical decision process.&quot;</rdfs:comment>
        <rdfs:label xml:lang="en">Previously Existing Process Evaluation Documentation</rdfs:label>
        <skos:definition xml:lang="en">Any related documentation or information about previously existing process being enhanced or replaced by the new process. This also includes information about the new process for the comparison purpose with the previously existing process.</skos:definition>
    </owl:Class>
    


    <!-- https://w3id.org/stav#PreviouslyExistingProcessKnownNegativeImpactInformation -->


    <owl:Class rdf:about="https://w3id.org/stav#PreviouslyExistingProcessKnownNegativeImpactInformation">
        <rdfs:subClassOf rdf:resource="http://www.w3.org/ns/odrl/2/Asset"/>
        <rdfs:label xml:lang="en">Previously Existing Process Known Negative Impact Information</rdfs:label>
        <skos:definition xml:lang="en">Any known harm, shortcoming, failure case, or material negative impact on consumers of the previously existing process used to make a decision.</skos:definition>
    </owl:Class>
    


    <!-- https://w3id.org/stav#PrivacyRisksAndPrivacyMeasuresEvaluationDocumentation -->


    <owl:Class rdf:about="https://w3id.org/stav#PrivacyRisksAndPrivacyMeasuresEvaluationDocumentation">
        <rdfs:subClassOf rdf:resource="http://www.w3.org/ns/odrl/2/AssetCollection"/>
        <rdfs:label xml:lang="en">Privacy Risks and Privacy Measures Evaluation Documentation</rdfs:label>
    </owl:Class>
    


    <!-- https://w3id.org/stav#ProductServiceDescription -->


    <owl:Class rdf:about="https://w3id.org/stav#ProductServiceDescription">
        <rdfs:subClassOf rdf:resource="http://www.w3.org/ns/odrl/2/Asset"/>
        <rdfs:comment xml:lang="en">Annex IV (1) (d) EU AI Act</rdfs:comment>
        <rdfs:label xml:lang="en">Product Service Descriptipn</rdfs:label>
        <skos:definition xml:lang="en">The description of the form in which the AI system is placed on the market or put into service.

One AI system can has more than one form of product or service.</skos:definition>
    </owl:Class>
    


    <!-- https://w3id.org/stav#ProductVisualImage -->


    <owl:Class rdf:about="https://w3id.org/stav#ProductVisualImage">
        <rdfs:subClassOf rdf:resource="http://www.w3.org/ns/odrl/2/Asset"/>
        <rdfs:comment xml:lang="en">Annex IV (1) (f) EU AI Act

(f) where the AI system is a component of products, photographs or illustrations showing external features, marking and internal layout of those products;</rdfs:comment>
        <rdfs:label xml:lang="en">Product Visual Image</rdfs:label>
        <skos:definition xml:lang="en">A photograph or an illustration showing external features, marking, and internal layout of a product that the AI system is part of.</skos:definition>
    </owl:Class>
    


    <!-- https://w3id.org/stav#PuttingIntoService -->


    <owl:Class rdf:about="https://w3id.org/stav#PuttingIntoService">
        <rdfs:subClassOf rdf:resource="http://www.w3.org/ns/odrl/2/Action"/>
        <rdfs:label xml:lang="en">putting into service</rdfs:label>
        <skos:definition xml:lang="en">‘putting into service’ means the supply of an AI system for first use directly to the user or for own use on the Union market for its intended purpose.</skos:definition>
        <skos:note xml:lang="en">Article 3 (11)</skos:note>
        <odrl:source>https://eur-lex.europa.eu/legal-content/EN/TXT/HTML/?uri=CELEX:52021PC0206&amp;from=EN</odrl:source>
    </owl:Class>
    


    <!-- https://w3id.org/stav#QualityManagementSystemDocumentationObligation -->


    <owl:Class rdf:about="https://w3id.org/stav#QualityManagementSystemDocumentationObligation">
        <rdfs:subClassOf rdf:resource="https://w3id.org/stap#InformationCreationObligation"/>
        <rdfs:label xml:lang="en">Quality Management System Documentation Obligation</rdfs:label>
        <skos:definition xml:lang="en">A quality management system ensures compliance of an AI system. A quality management system documentation shall be in the form of written policies, procedures and instructions. It shall include a strategy for regulatory compliance; techniques, procedures and systematic actions to be used for the design, development, and examination of the AI system, etc.</skos:definition>
    </owl:Class>
    


    <!-- https://w3id.org/stav#RealWorldConditionsTestingPlan -->


    <owl:Class rdf:about="https://w3id.org/stav#RealWorldConditionsTestingPlan">
        <rdfs:subClassOf rdf:resource="http://www.w3.org/ns/odrl/2/Asset"/>
        <rdfs:comment xml:lang="en">A summary of the main characteristics of the plan for testing in real world conditions.</rdfs:comment>
        <rdfs:label xml:lang="en">Real World Conditions Testing Plan</rdfs:label>
        <skos:note xml:lang="en">EU AI Act Annex VIIIa (4)</skos:note>
    </owl:Class>
    


    <!-- https://w3id.org/stav#RealWorldConditionsTestingSuspensionOrTerminationInformation -->


    <owl:Class rdf:about="https://w3id.org/stav#RealWorldConditionsTestingSuspensionOrTerminationInformation">
        <rdfs:subClassOf rdf:resource="http://www.w3.org/ns/odrl/2/Asset"/>
        <rdfs:comment xml:lang="en">Information on the suspension or termination of the testing in real world conditions.</rdfs:comment>
        <rdfs:label xml:lang="en">Real World Conditions Testing Suspension Or Termination Information</rdfs:label>
        <skos:note xml:lang="en">EU AI Act Annex VIIIa (5)</skos:note>
    </owl:Class>
    


    <!-- https://w3id.org/stav#RealWorldConditionsTestingUser -->


    <owl:Class rdf:about="https://w3id.org/stav#RealWorldConditionsTestingUser">
        <rdfs:subClassOf rdf:resource="http://www.w3.org/ns/odrl/2/Party"/>
        <rdfs:comment xml:lang="en">users involved in the testing in real world conditions.</rdfs:comment>
        <rdfs:label xml:lang="en">Real World Conditions Testing User</rdfs:label>
        <skos:note xml:lang="en">EU AI Act Annex VIIIa (2)</skos:note>
    </owl:Class>
    


    <!-- https://w3id.org/stav#RegisterationObligation -->


    <owl:Class rdf:about="https://w3id.org/stav#RegisterationObligation">
        <rdfs:subClassOf rdf:resource="https://w3id.org/stap#InformationSubmissionObligation"/>
        <rdfs:label xml:lang="en">Registeration Obligation</rdfs:label>
        <skos:definition xml:lang="en">A registration to a database containing information about AI systems.</skos:definition>
    </owl:Class>
    


    <!-- https://w3id.org/stav#RiskManagementSystemDescription -->


    <owl:Class rdf:about="https://w3id.org/stav#RiskManagementSystemDescription">
        <rdfs:subClassOf rdf:resource="http://www.w3.org/ns/odrl/2/Asset"/>
        <rdfs:label xml:lang="en">Risk Management System Description</rdfs:label>
    </owl:Class>
    


    <!-- https://w3id.org/stav#SoftwareDependencies -->


    <owl:Class rdf:about="https://w3id.org/stav#SoftwareDependencies">
        <rdfs:subClassOf rdf:resource="http://www.w3.org/ns/odrl/2/Asset"/>
        <rdfs:comment xml:lang="en">Annex IV (1) (c) EU AI Act

This is the area that Software Bill of Materials can help a lot.

&quot;versions of relevant software or firmware&quot; can taken from software metadata that package manager already have.

The &quot;any requirement related to version update&quot; could be a narrative one and need further clarification.</rdfs:comment>
        <rdfs:label xml:lang="en">Software Dependencies</rdfs:label>
        <skos:definition xml:lang="en">The versions of relevant software or firmware and any requirement related to version update.</skos:definition>
    </owl:Class>
    


    <!-- https://w3id.org/stav#SystemDetailedDescription -->


    <owl:Class rdf:about="https://w3id.org/stav#SystemDetailedDescription">
        <rdfs:subClassOf rdf:resource="http://www.w3.org/ns/odrl/2/AssetCollection"/>
        <rdfs:label xml:lang="en">System Detailed Description</rdfs:label>
    </owl:Class>
    


    <!-- https://w3id.org/stav#SystemEvaluationDocumentation -->


    <owl:Class rdf:about="https://w3id.org/stav#SystemEvaluationDocumentation">
        <rdfs:subClassOf rdf:resource="http://www.w3.org/ns/odrl/2/AssetCollection"/>
        <rdfs:label>System Evaluation Documentation</rdfs:label>
    </owl:Class>
    


    <!-- https://w3id.org/stav#SystemGeneralDescription -->


    <owl:Class rdf:about="https://w3id.org/stav#SystemGeneralDescription">
        <rdfs:subClassOf rdf:resource="http://www.w3.org/ns/odrl/2/AssetCollection"/>
        <rdfs:comment xml:lang="en">Similar to what defined in Annex IV (1) of EU AI Act,
as part of the Technical Documentation referred to in Article 11 (1)</rdfs:comment>
        <rdfs:label xml:lang="en">System General Description</rdfs:label>
        <skos:definition xml:lang="en">A general description of the AI system.</skos:definition>
    </owl:Class>
    


    <!-- https://w3id.org/stav#TechnicalDocumentation -->


    <owl:Class rdf:about="https://w3id.org/stav#TechnicalDocumentation">
        <rdfs:subClassOf rdf:resource="http://www.w3.org/ns/odrl/2/AssetCollection"/>
        <rdfs:comment xml:lang="en">Similar to &quot;Transparency Report&quot;
as defined in Sec. 203. (a) (2) of
S.3312 - Artificial Intelligence Research, Innovation, and Accountability Act of 2023
https://www.govtrack.us/congress/bills/118/s3312/text/is#link=II_203_a_2</rdfs:comment>
        <rdfs:label xml:lang="en">Technical Documentation</rdfs:label>
        <skos:definition xml:lang="en">The technical documentation shall be drawn up in such a way to demonstrate that the high-risk AI system complies with the requirements set out in Title III Chapter 2 and provide national competent authorities and notified bodies with all the necessary information to assess the compliance of the AI system with those requirements. It shall contain, at a minimum, the elements set out in Annex IV.</skos:definition>
        <skos:note>Article 11</skos:note>
        <odrl:source>https://eur-lex.europa.eu/legal-content/EN/TXT/HTML/?uri=CELEX:52021PC0206&amp;from=EN</odrl:source>
    </owl:Class>
    


    <!-- https://w3id.org/stav#TechnicalDocumentationObligation -->


    <owl:Class rdf:about="https://w3id.org/stav#TechnicalDocumentationObligation">
        <rdfs:subClassOf rdf:resource="https://w3id.org/stap#InformationCreationObligation"/>
        <rdfs:label xml:lang="en">Technical Documentation Obligation</rdfs:label>
        <skos:definition xml:lang="en">The technical documentation of an AI system contains information including its intended purpose and limitations, risk management process, data governance, and instructions of use.</skos:definition>
    </owl:Class>
</rdf:RDF>



<!-- Generated by the OWL API (version 5.1.18) https://github.com/owlcs/owlapi/ -->


